\subsection{Additive Expression}

\begin{grammar}
\nonterminal{additive-expression}
    \produces
	\nonterminal{multiplicative-expression} \\
    \produces
	\nonterminal{additive-expression}
	\lexkeyword{+}
	\nonterminal{multiplicative-expression} \\
    \produces
	\nonterminal{additive-expression}
	\lexkeyword{-}
	\nonterminal{multiplicative-expression} \\
\end{grammar}

\subsubsection{Eliminating left recursion}

Eliminating left recursion leads to
\begin{grammar}
\underbrace{\nonterminal{additive-expression}}_{=: A}
    \produces
	\underbrace{\nonterminal{multiplicative-expression}}_{=: M}
	\underbrace{\nonterminal{additive-expression'}}_{=:A'}\\
\nonterminal{additive-expression'}
    \produces
	\lexkeyword{+}
	\nonterminal{multiplicative-expression}
	\nonterminal{additive-expression'}
	\\
    \produces
	\lexkeyword{-}
	\nonterminal{multiplicative-expression}
	\nonterminal{additive-expression'}
	\\
    \produces
\end{grammar}\\[-0.5cm]
\noindent
The left associativity of the operators \lexkeyword{+} and \lexkeyword{-} needs
to be handled manually by the parser.

\paragraph{Item automata for A}


\[
\begin{tikzpicture}[
    every text node part/.style={align=center},
    initial text =
]
    \node[state,initial]
	(S)[rounded rectangle, draw]
	{{$[A\to .MA']$}};
    \node[state]
	(M)[rounded rectangle, draw,right=of S]
	{{$[A\to M.A']$}};
    \node[state,accepting]
	(A_)[rounded rectangle, draw,right=of M]
	{{$[A\to MA'.]$}};
    \path[->] (S) edge  node [above] {M} (M);
    \path[->] (M) edge  node [above] {A'} (A_);
\end{tikzpicture}
\]

\paragraph{Item automata for A'}
\[
\begin{tikzpicture}[
    every text node part/.style={align=center},
    initial text =
]
    \node[state,initial,accepting]
	(S)[rounded rectangle, draw]
	{
	    {$[A'\to .+MA']$}\\
	    {$[A'\to .-MA']$}\\
	    {$[A'\to .]$}
	};
    \node[state]
	(Add)[rounded rectangle, draw,right=of S]
	{{$[A'\to +.MA']$}};
    \node[state]
	(Sub)[rounded rectangle, draw,below=of Add]
	{{$[A'\to -.MA']$}};
    \node[state]
	(M)[rounded rectangle, draw,right=of Add]
	{
	    {$[A'\to +M.A']$} \\
	    {$[A'\to -M.A']$}
	};
    \node[state,accepting]
	(E)[rounded rectangle, draw,right=of M]
	{
	    {$[A'\to +MA'.]$} \\
	    {$[A'\to -MA'.]$}
	};
    \path[->] (S) edge  node [above] {\lexkeyword{+}} (Add);
    \path[->] (S) edge  node [above] {\lexkeyword{-}} (Sub);
    \path[->] (Add) edge  node [above] {M} (M);
    \path[->] (Sub) edge  node [above] {M} (M);
    \path[->] (M) edge  node [above] {A'} (E);
\end{tikzpicture}
\]

\subsubsection{Eliminating left recursion (in EBNF Form)}

Expressing the BNF notation in EBNF reveals how the item automata for $A$ and
$A'$ can be combined in an implementation using a while loop
checking if the
current token is in $\mathrm{First}(A') = \{ \lexkeyword{+}, \lexkeyword{-}\}$:
\begin{grammar}
\underbrace{\nonterminal{additive-expression}}_{= A}
    \produces
	\underbrace{\nonterminal{multiplicative-expression}}_{= M}
	\underbrace{
	\{\;
	    \nonterminal{additive-op}
	    \nonterminal{multiplicative-expression}
	\}
	}_{=A'}
	\\
\nonterminal{additive-op}
    \produces
    \lexkeyword{+} \\
    \produces
    \lexkeyword{-} \\
\end{grammar}\\[-0.5cm]

