\subsection{Expression sequence}

\begin{grammar}
\underbrace{\nonterminal{expression-sequence}}_{=:S}
    \produces
	\underbrace{\nonterminal{expression}}_{=:E} \\
    \produces
	\nonterminal{expression-sequence}
	\nonterminal{expression} \\
\end{grammar}

\subsubsection{Eliminating left recursion}

\begin{grammar}
\underbrace{\nonterminal{expression-sequence}}_{=:S}
    \produces
	\underbrace{\nonterminal{expression}}_{=:E}
	\underbrace{\nonterminal{expression-sequence'}}_{=:S'} \\
\nonterminal{expression-sequence'}
    \produces
	\nonterminal{expression}
	\nonterminal{expression-sequence'}
	\\
    \produces
\end{grammar}


\paragraph{Item automata for S}
\[
\begin{tikzpicture}[
    every text node part/.style={align=center},
    initial text =
]
    \node[state,initial]
	(S)[rounded rectangle, draw]
	{
	    {$[S \to .ES']$}
	};
    \node[state]
	(E)[rounded rectangle, draw, right=of S]
	{
	    {$[S \to E.S']$}
	};
    \node[state]
	(End)[rounded rectangle, draw, right=of E]
	{
	    {$[S \to ES'.]$}
	};

    \path[->] (S) edge  node [above] {E} (E);
    \path[->] (E) edge  node [above] {S'} (End);
\end{tikzpicture}
\]
\paragraph{Item automata for S'}
\[
\begin{tikzpicture}[
    every text node part/.style={align=center},
    initial text =
]
    \node[state,initial,accepting]
	(S)[rounded rectangle, draw]
	{
	    {$[S'\to .*ES']$}\\
	    {$[S'\to .]$}
	};
    \node[state]
	(E)[rounded rectangle, draw,right=of S]
	{
	    {$[S'\to E.S']$}
	};
    \node[state,accepting]
	(End)[rounded rectangle, draw,right=of E]
	{
	    {$[S'\to ES'.]$}
	};
    \path[->] (S) edge  node [above] {E} (E);
    \path[->] (E) edge  node [above] {S'} (End);
\end{tikzpicture}
\]


\subsubsection{Eliminating left recursion (in EBNF Form)}

Expressing the BNF notation in EBNF reveals how the item automata for $S$ and
$S'$ can be combined in an implementation using a do-while loop:

\begin{grammar}
\underbrace{\nonterminal{expression-sequence}}_{= S}
    \produces
	\underbrace{\nonterminal{expression}}_{= E}
	\underbrace{
	\{\;
	    \nonterminal{expression}
	\}
	}_{= E'}
	\\
\end{grammar}\\[-0.5cm]
In the case the loop can terminate if the current token is
$\mathrm{Follow}(E') = \{ \lexkeyword{EOI} \}$.

