\subsection{Multiplicative Expression}

\begin{grammar}
\nonterminal{multiplicative-expression}
    \produces
	\nonterminal{power-expression} \\
    \produces
	\nonterminal{multiplicative-expression}
	\lexkeyword{*}
	\nonterminal{power-expression} \\
    \produces
	\nonterminal{multiplicative-expression}
	\lexkeyword{/}
	\nonterminal{power-expression} \\
\end{grammar}

\subsubsection{Eliminating left recursion (in BNF Form)}

Eliminating left recursion leads to
\begin{grammar}
\underbrace{\nonterminal{multiplicative-expression}}_{=: M}
    \produces
	\underbrace{\nonterminal{power-expression}}_{=: P}
	\underbrace{\nonterminal{multiplicative-expression'}}_{=:M'}\\
\nonterminal{multiplicative-expression'}
    \produces
	\lexkeyword{*}
	\nonterminal{power-expression} \nonterminal{multiplicative-expression'}
	\\
    \produces
	\lexkeyword{/}
	\nonterminal{power-expression} \nonterminal{multiplicative-expression'}
	\\
    \produces
\end{grammar}\\[-0.5cm]
\noindent

\paragraph{Item automata for M}

\[
\begin{tikzpicture}[
    every text node part/.style={align=center},
    initial text =
]
    \node[state,initial]
	(S)[rounded rectangle, draw]
	{{$[M\to .PM']$}};
    \node[state]
	(P)[rounded rectangle, draw,right=of S]
	{{$[M\to P.M']$}};
    \node[state,accepting]
	(M_)[rounded rectangle, draw,right=of P]
	{{$[M\to PM'.]$}};
    \path[->] (S) edge  node [above] {P} (P);
    \path[->] (P) edge  node [above] {M'} (M_);
\end{tikzpicture}
\]

\paragraph{Item automata for M'}
\[
\begin{tikzpicture}[
    every text node part/.style={align=center},
    initial text =
]
    \node[state,initial,accepting]
	(S)[rounded rectangle, draw]
	{
	    {$[M'\to .*PM']$}\\
	    {$[M'\to ./PM']$}\\
	    {$[M'\to .]$}
	};
    \node[state]
	(Mul)[rounded rectangle, draw,right=of S]
	{{$[M'\to *.PM']$}};
    \node[state]
	(Div)[rounded rectangle, draw,below=of Mul]
	{{$[M'\to /.PM']$}};
    \node[state]
	(P)[rounded rectangle, draw,right=of Mul]
	{
	    {$[M'\to *P.M']$} \\
	    {$[M'\to /P.M']$}
	};
    \node[state,accepting]
	(E)[rounded rectangle, draw,right=of P]
	{
	    {$[M'\to *PM'.]$} \\
	    {$[M'\to /PM'.]$}
	};
    \path[->] (S) edge  node [above] {\lexkeyword{*}} (Mul);
    \path[->] (S) edge  node [above] {\lexkeyword{/}} (Div);
    \path[->] (Mul) edge  node [above] {P} (P);
    \path[->] (Div) edge  node [above] {P} (P);
    \path[->] (P) edge  node [above] {M'} (E);
\end{tikzpicture}
\]

\subsubsection{Eliminating left recursion (in EBNF Form)}

Expressing the BNF notation in EBNF reveals how the item automata for $M$ and
$M'$ can be combined in an implementation using a while loop
checking if the
current token is in $\mathrm{First}(M') = \{ \lexkeyword{*}, \lexkeyword{/}\}$:
\begin{grammar}
\underbrace{\nonterminal{multiplicative-expression}}_{= M}
    \produces
	\underbrace{\nonterminal{power-expression}}_{= P}
	\{\;
	\underbrace{
	    \nonterminal{multiplicative-op}
	    \nonterminal{power-expression}
	    }_{=M'}
	\}
	\\
\nonterminal{multiplicative-op}
    \produces
    \lexkeyword{*} \\
    \produces
    \lexkeyword{/} \\
\end{grammar}\\[-0.5cm]

